src/opt_common/ReorderRelFenceCommon.v
@@ -1,0 +1,409 @@
+From sflib Require Import sflib.
+From Paco Require Import paco.
+
+From PromisingLib Require Import Axioms.
+From PromisingLib Require Import Basic.
+From PromisingLib Require Import Loc.
+From PromisingLib Require Import Language.
+
+Require Import Event.
+Require Import Time.
+Require Import View.
+Require Import Cell.
+Require Import Memory.
+Require Import TView.
+Require Import Local.
+Require Import Thread.
+Require Import Configuration.
+Require Import Progress.
+
+Require Import SimMemory.
+Require Import SimPromises.
+Require Import SimLocal.
+Require Import SimThread.
+
+Require Import FulfillStep.
+Require Import ReorderStep.
+
+Set Implicit Arguments.
+
+
+Definition local_relfenced (lc:Local.t) :=
+  (Local.mk (TView.mk
+               (fun _ => (TView.cur (Local.tview lc)))
+               (TView.cur (Local.tview lc))
+               (TView.acq (Local.tview lc)))
+            (Local.promises lc)).
+
+Lemma local_relfenced_wf
+      lc mem
+      (WF: Local.wf lc mem):
+  Local.wf (local_relfenced lc) mem.
+Proof.
+  inv WF. econs; ss; eauto.
+  - inv TVIEW_WF. econs; ss. refl.
+  - inv TVIEW_CLOSED. econs; ss.
+Qed.
+
+Lemma sim_local_promise_relfenced
+      pview
+      lc1_src mem1_src
+      lc1_tgt mem1_tgt
+      lc2_tgt mem2_tgt
+      loc from to msg kind
+      (STEP_TGT: Local.promise_step lc1_tgt mem1_tgt loc from to msg lc2_tgt mem2_tgt kind)
+      (LOCAL1: sim_local pview lc1_src (local_relfenced lc1_tgt))
+      (MEM1: sim_memory mem1_src mem1_tgt)
+      (WF1_SRC: Local.wf lc1_src mem1_src)
+      (WF1_TGT: Local.wf lc1_tgt mem1_tgt)
+      (MEM1_SRC: Memory.closed mem1_src)
+      (MEM1_TGT: Memory.closed mem1_tgt):
+  exists lc2_src mem2_src,
+    <<STEP_SRC: Local.promise_step lc1_src mem1_src loc from to (SimPromises.none_if loc to pview msg) lc2_src mem2_src (SimPromises.kind_transf loc to pview kind)>> /\
+    <<LOCAL2: sim_local pview lc2_src (local_relfenced lc2_tgt)>> /\
+    <<MEM2: sim_memory mem2_src mem2_tgt>>.
+Proof.
+  inv LOCAL1. inv STEP_TGT.
+  exploit SimPromises.promise; eauto.
+  { apply WF1_SRC. }
+  { apply WF1_TGT. }
+  i. des.
+  exploit Memory.promise_future; try apply PROMISE_SRC; try apply WF1_SRC; eauto.
+  { SimPromises.none_if_tac; econs; ss. inv CLOSED.
+    eapply sim_memory_closed_opt_view; eauto. }
+  i. des.
+  esplits; eauto.
+  - econs; eauto.
+    SimPromises.none_if_tac; econs; ss. inv CLOSED.
+    eapply sim_memory_closed_opt_view; eauto.
+  - econs; eauto.
+Qed.
+
+Lemma sim_local_read_relfenced
+      pview
+      lc1_src mem1_src
+      lc1_tgt mem1_tgt
+      lc2_tgt
+      loc ts val released_tgt ord_src ord_tgt
+      (STEP_TGT: Local.read_step lc1_tgt mem1_tgt loc ts val released_tgt ord_tgt lc2_tgt)
+      (LOCAL1: sim_local pview lc1_src (local_relfenced lc1_tgt))
+      (MEM1: sim_memory mem1_src mem1_tgt)
+      (WF1_SRC: Local.wf lc1_src mem1_src)
+      (WF1_TGT: Local.wf lc1_tgt mem1_tgt)
+      (MEM1_SRC: Memory.closed mem1_src)
+      (MEM1_TGT: Memory.closed mem1_tgt)
+      (ORD: Ordering.le ord_src ord_tgt):
+  exists released_src lc2_src,
+    <<REL: View.opt_le released_src released_tgt>> /\
+    <<STEP_SRC: Local.read_step lc1_src mem1_src loc ts val released_src ord_src lc2_src>> /\
+    <<LOCAL2: sim_local pview lc2_src (local_relfenced lc2_tgt)>>.
+Proof.
+  inv LOCAL1. inv STEP_TGT.
+  exploit sim_memory_get; try apply GET; try apply MEM1. i. des. inv MSG.
+  esplits; eauto.
+  - econs; eauto. eapply TViewFacts.readable_mon; eauto. apply TVIEW.
+  - econs; eauto. inv TVIEW. ss. econs; s.
+    + i. unfold LocFun.find. etrans; [by apply WF1_SRC|].
+      eauto using View.join_l.
+    + repeat apply View.join_le; ss.
+      * unfold View.singleton_ur_if. repeat condtac; viewtac.
+      * repeat condtac; viewtac.
+    + repeat apply View.join_le; ss.
+      * unfold View.singleton_ur_if. repeat condtac; viewtac.
+      * repeat condtac; viewtac.
+Qed.
+
+Lemma sim_local_fulfill_relfenced
+      pview
+      lc1_src sc1_src mem1_src
+      lc1_tgt sc1_tgt mem1_tgt
+      lc2_tgt sc2_tgt
+      loc from to val releasedm_src releasedm_tgt released ord_src ord_tgt
+      (RELM_LE: View.opt_le releasedm_src releasedm_tgt)
+      (RELM_WF: View.opt_wf releasedm_src)
+      (RELM_CLOSED: Memory.closed_opt_view releasedm_src mem1_src)
+      (WF_RELM_TGT: View.opt_wf releasedm_tgt)
+      (ORD: Ordering.le ord_src ord_tgt)
+      (PVIEW: (Ordering.le Ordering.acqrel ord_tgt /\ SimPromises.mem loc to pview = false) \/
+              Ordering.le ord_tgt Ordering.plain)
+      (STEP_TGT: fulfill_step lc1_tgt sc1_tgt loc from to val releasedm_tgt released ord_tgt lc2_tgt sc2_tgt)
+      (LOCAL1: sim_local pview lc1_src (local_relfenced lc1_tgt))
+      (SC1: TimeMap.le sc1_src sc1_tgt)
+      (MEM1: sim_memory mem1_src mem1_tgt)
+      (WF1_SRC: Local.wf lc1_src mem1_src)
+      (WF1_TGT: Local.wf lc1_tgt mem1_tgt)
+      (SC1_SRC: Memory.closed_timemap sc1_src mem1_src)
+      (SC1_TGT: Memory.closed_timemap sc1_tgt mem1_tgt)
+      (MEM1_SRC: Memory.closed mem1_src)
+      (MEM1_TGT: Memory.closed mem1_tgt):
+  exists lc2_src sc2_src,
+    <<STEP_SRC: fulfill_step lc1_src sc1_src loc from to val releasedm_src (SimPromises.none_if_released loc to pview released) ord_src lc2_src sc2_src>> /\
+    <<LOCAL2: sim_local (SimPromises.unset loc to pview) lc2_src (local_relfenced lc2_tgt)>> /\
+    <<SC2: TimeMap.le sc2_src sc2_tgt>>.
+Proof.
+  guardH PVIEW.
+  inv STEP_TGT.
+  assert (RELT_LE:
+   View.opt_le
+     (TView.write_released (Local.tview lc1_src) sc1_src loc to releasedm_src ord_src)
+     (TView.write_released (Local.tview lc1_tgt) sc2_tgt loc to releasedm_tgt ord_tgt)).
+  { unguardH PVIEW. des.
+    - unfold TView.write_released.
+      condtac; [|by econs].
+      condtac; cycle 1.
+      { by destruct ord_src, ord_tgt; inv PVIEW; inv COND0. }
+      econs. unfold TView.write_tview. s.
+      repeat (condtac; aggrtac); try by apply WF1_TGT.
+      + rewrite <- View.join_r. rewrite <- ? View.join_l. apply LOCAL1.
+      + rewrite <- View.join_r. rewrite <- ? View.join_l.
+        etrans; [|apply LOCAL1]. apply WF1_SRC.
+    - unfold TView.write_released. repeat (condtac; viewtac).
+  }
+  assert (RELT_WF:
+   View.opt_wf (TView.write_released (Local.tview lc1_src) sc1_src loc to releasedm_src ord_src)).
+  { unfold TView.write_released. condtac; econs.
+    repeat (try condtac; viewtac; try apply WF1_SRC).
+  }
+  exploit SimPromises.remove; try exact REMOVE;
+    try exact MEM1; try apply LOCAL1; eauto.
+  { econs. ss. }
+  { apply WF1_SRC. }
+  { apply WF1_TGT. }
+  { apply WF1_TGT. }
+  i. des. esplits.
+  - econs; eauto.
+    + unfold SimPromises.none_if_released. condtac.
+      * unguardH PVIEW. des; ss. unfold TView.write_released. condtac; [|refl].
+        destruct ord_src, ord_tgt; inv ORD; inv PVIEW; inv COND0.
+      * etrans; eauto.
+    + unfold SimPromises.none_if_released. condtac; viewtac.
+    + eapply TViewFacts.writable_mon; try exact WRITABLE; eauto. apply LOCAL1.
+  - econs; eauto. inv LOCAL1. inv TVIEW. ss. econs; s.
+    + i. rewrite LocFun.add_spec. condtac; ss.
+      { subst. unfold LocFun.find. condtac; apply View.join_le; viewtac.
+        etrans; eauto. refl.
+      }
+      unfold LocFun.find. etrans; [by apply WF1_SRC|].
+      eauto using View.join_l.
+    + apply View.join_le; viewtac.
+    + apply View.join_le; viewtac.
+  - ss.
+Qed.
+
+Lemma sim_local_promise_not_lower
+      pview
+      lc1_src
+      lc1_tgt mem1_tgt loc from to msg_tgt lc1 mem2_tgt kind
+      (LOCAL: sim_local pview lc1_src (local_relfenced lc1_tgt))
+      (STEP: Local.promise_step lc1_tgt mem1_tgt loc from to msg_tgt lc1 mem2_tgt kind)
+      (KIND: negb (Memory.op_kind_is_lower kind)):
+  SimPromises.mem loc to pview = false.
+Proof.
+  destruct (SimPromises.mem loc to pview) eqn:X; ss.
+  inv LOCAL. inv PROMISES. exploit PVIEW; eauto. i.
+  inv STEP. inv PROMISE; ss.
+  - exploit Memory.add_get0; try exact PROMISES; eauto. i. des. congr.
+  - exploit Memory.split_get0; try exact PROMISES; eauto. i. des. congr.
+  - exploit Memory.remove_get0; try exact PROMISES; eauto. i. des. congr.
+Qed.
+
+Lemma sim_local_write_relfenced
+      pview
+      lc1_src sc1_src mem1_src
+      lc1_tgt sc1_tgt mem1_tgt
+      lc2_tgt sc2_tgt mem2_tgt
+      loc from to val releasedm_src releasedm_tgt released_tgt ord_src ord_tgt kind
+      (RELM_LE: View.opt_le releasedm_src releasedm_tgt)
+      (RELM_SRC_WF: View.opt_wf releasedm_src)
+      (RELM_SRC_CLOSED: Memory.closed_opt_view releasedm_src mem1_src)
+      (RELM_TGT_WF: View.opt_wf releasedm_tgt)
+      (RELM_TGT_CLOSED: Memory.closed_opt_view releasedm_tgt mem1_tgt)
+      (ORD: Ordering.le ord_src ord_tgt)
+      (ORD_TGT: Ordering.le ord_tgt Ordering.plain \/ Ordering.le Ordering.acqrel ord_tgt)
+      (STEP_TGT: Local.write_step lc1_tgt sc1_tgt mem1_tgt loc from to val releasedm_tgt released_tgt ord_tgt lc2_tgt sc2_tgt mem2_tgt kind)
+      (LOCAL1: sim_local pview lc1_src (local_relfenced lc1_tgt))
+      (SC1: TimeMap.le sc1_src sc1_tgt)
+      (MEM1: sim_memory mem1_src mem1_tgt)
+      (WF1_SRC: Local.wf lc1_src mem1_src)
+      (WF1_TGT: Local.wf lc1_tgt mem1_tgt)
+      (SC1_SRC: Memory.closed_timemap sc1_src mem1_src)
+      (SC1_TGT: Memory.closed_timemap sc1_tgt mem1_tgt)
+      (MEM1_SRC: Memory.closed mem1_src)
+      (MEM1_TGT: Memory.closed mem1_tgt):
+  exists released_src lc2_src sc2_src mem2_src,
+    <<STEP_SRC: Local.write_step lc1_src sc1_src mem1_src loc from to val releasedm_src released_src ord_src lc2_src sc2_src mem2_src (SimPromises.kind_transf loc to pview kind)>> /\
+    <<REL2: View.opt_le released_src released_tgt>> /\
+    <<LOCAL2: sim_local (SimPromises.unset loc to pview) lc2_src (local_relfenced lc2_tgt)>> /\
+    <<SC2: TimeMap.le sc2_src sc2_tgt>> /\
+    <<MEM2: sim_memory mem2_src mem2_tgt>>.
+Proof.
+  guardH ORD_TGT.
+  exploit write_promise_fulfill; eauto. i. des.
+  exploit Local.promise_step_future; eauto. i. des.
+  exploit sim_local_promise_relfenced; eauto. i. des.
+  exploit Local.promise_step_future; eauto. i. des.
+  assert (PVIEW: __guard__ ((Ordering.le Ordering.acqrel ord_tgt /\ SimPromises.mem loc to pview = false) \/
+                              Ordering.le ord_tgt Ordering.plain)).
+  { destruct (Ordering.le ord_tgt Ordering.strong_relaxed) eqn:X.
+    - right. unguardH ORD_TGT. destruct ord_tgt; des; ss.
+    - left. splits.
+      { by destruct ord_tgt; inv X. }
+      hexploit ORD0.
+      { by destruct ord_tgt; inv X. }
+      exploit Local.write_step_strong_relaxed; eauto.
+      { by destruct ord_tgt. }
+      i. eapply sim_local_promise_not_lower; try exact STEP1; eauto.
+  }
+  exploit sim_local_fulfill_relfenced; try apply STEP2;
+    try apply LOCAL2; try apply MEM2; eauto.
+  { eapply Memory.future_closed_opt_view; eauto. }
+  i. des.
+  exploit promise_fulfill_write_sim_memory; try exact STEP_SRC; try exact STEP_SRC0; eauto.
+  { i. hexploit ORD0; eauto.
+    i. des. subst. splits; auto. eapply sim_local_nonsynch_loc; eauto.
+  }
+  i. des. esplits; eauto.
+  - unguardH PVIEW. des.
+    + unfold SimPromises.none_if_released in *. rewrite PVIEW0 in *. ss.
+    + subst. unfold TView.write_released at 1. condtac; [|by econs].
+      destruct ord_src, ord_tgt; inv ORD; inv PVIEW; inv COND.
+  - etrans; eauto.
+Qed.
+
+Lemma sim_local_update_relfenced
+      pview
+      lc1_src sc1_src mem1_src
+      lc1_tgt sc1_tgt mem1_tgt
+      lc2_tgt
+      lc3_tgt sc3_tgt mem3_tgt
+      loc ts1 val1 released1_tgt ord1_src ord1_tgt
+      from2 to2 val2 released2_tgt ord2_src ord2_tgt kind
+      (STEP1_TGT: Local.read_step lc1_tgt mem1_tgt loc ts1 val1 released1_tgt ord1_tgt lc2_tgt)
+      (STEP2_TGT: Local.write_step lc2_tgt sc1_tgt mem1_tgt loc from2 to2 val2 released1_tgt released2_tgt ord2_tgt lc3_tgt sc3_tgt mem3_tgt kind)
+      (LOCAL1: sim_local pview lc1_src (local_relfenced lc1_tgt))
+      (SC1: TimeMap.le sc1_src sc1_tgt)
+      (MEM1: sim_memory mem1_src mem1_tgt)
+      (WF1_SRC: Local.wf lc1_src mem1_src)
+      (WF1_TGT: Local.wf lc1_tgt mem1_tgt)
+      (SC1_SRC: Memory.closed_timemap sc1_src mem1_src)
+      (SC1_TGT: Memory.closed_timemap sc1_tgt mem1_tgt)
+      (MEM1_SRC: Memory.closed mem1_src)
+      (MEM1_TGT: Memory.closed mem1_tgt)
+      (ORD1: Ordering.le ord1_src ord1_tgt)
+      (ORD2: Ordering.le ord2_src ord2_tgt)
+      (ORD2_TGT: Ordering.le ord2_tgt Ordering.plain \/ Ordering.le Ordering.acqrel ord2_tgt):
+  exists released1_src released2_src lc2_src lc3_src sc3_src mem3_src,
+    <<REL1: View.opt_le released1_src released1_tgt>> /\
+    <<REL2: View.opt_le released2_src released2_tgt>> /\
+    <<STEP1_SRC: Local.read_step lc1_src mem1_src loc ts1 val1 released1_src ord1_src lc2_src>> /\
+    <<STEP2_SRC: Local.write_step lc2_src sc1_src mem1_src loc from2 to2 val2 released1_src released2_src ord2_src lc3_src sc3_src mem3_src (SimPromises.kind_transf loc to2 pview kind)>> /\
+    <<LOCAL3: sim_local (SimPromises.unset loc to2 pview) lc3_src (local_relfenced lc3_tgt)>> /\
+    <<SC3: TimeMap.le sc3_src sc3_tgt>> /\
+    <<MEM3: sim_memory mem3_src mem3_tgt>>.
+Proof.
+  guardH ORD2_TGT.
+  exploit Local.read_step_future; eauto. i. des.
+  exploit sim_local_read_relfenced; eauto. i. des.
+  exploit Local.read_step_future; eauto. i. des.
+  hexploit sim_local_write_relfenced; eauto. i. des.
+  esplits; eauto.
+Qed.
+
+Lemma sim_local_fence_relfenced
+      pview
+      lc1_src sc1_src mem1_src
+      lc1_tgt sc1_tgt mem1_tgt
+      lc2_tgt sc2_tgt
+      ordr_src ordw_src
+      ordr_tgt ordw_tgt
+      (STEP_TGT: Local.fence_step lc1_tgt sc1_tgt ordr_tgt ordw_tgt lc2_tgt sc2_tgt)
+      (LOCAL1: sim_local pview lc1_src (local_relfenced lc1_tgt))
+      (SC1: TimeMap.le sc1_src sc1_tgt)
+      (MEM1: sim_memory mem1_src mem1_tgt)
+      (WF1_SRC: Local.wf lc1_src mem1_src)
+      (WF1_TGT: Local.wf lc1_tgt mem1_tgt)
+      (ORDR: Ordering.le ordr_src ordr_tgt)
+      (ORDW: Ordering.le ordw_src ordw_tgt)
+      (ORDR_TGT: Ordering.le ordr_tgt Ordering.acqrel)
+      (ORDW_TGT: Ordering.le ordw_tgt Ordering.relaxed):
+  exists lc2_src sc2_src,
+    <<STEP_SRC: Local.fence_step lc1_src sc1_src ordr_src ordw_src lc2_src sc2_src>> /\
+    <<LOCAL2: sim_local pview lc2_src (local_relfenced lc2_tgt)>> /\
+    <<SC2: TimeMap.le sc2_src sc2_tgt>>.
+Proof.
+  inv STEP_TGT. esplits; eauto.
+  - econs; eauto.
+    + i. eapply sim_local_nonsynch; eauto.
+    + i. subst. eapply sim_local_memory_bot; eauto.
+      eapply PROMISES; eauto. destruct ordw_tgt; ss.
+  - inv LOCAL1. inv TVIEW. econs; ss.
+    econs; s; unfold LocFun.find; repeat condtac; aggrtac.
+    + etrans; eauto. apply WF1_TGT.
+    + etrans; eauto. apply WF1_TGT.
+    + etrans; eauto. apply WF1_TGT.
+  - unfold TView.write_fence_sc.
+    repeat (condtac; viewtac).
+Qed.
+
+Lemma sim_local_intro_relfenced
+      pview
+      lc1_src sc1_src mem1_src
+      lc1_tgt sc1_tgt mem1_tgt
+      (LOCAL1: sim_local pview lc1_src lc1_tgt)
+      (SC1: TimeMap.le sc1_src sc1_tgt)
+      (MEM1: sim_memory mem1_src mem1_tgt)
+      (WF1_SRC: Local.wf lc1_src mem1_src)
+      (WF1_TGT: Local.wf lc1_tgt mem1_tgt):
+  <<LOCAL2: sim_local pview lc1_src (local_relfenced lc1_tgt)>>.
+Proof.
+  esplits. inv LOCAL1. econs; eauto.
+  inv TVIEW. econs; ss; eauto.
+  etrans; eauto. apply WF1_TGT.
+Qed.
+
+Lemma sim_local_fence_src_relfenced
+      pview
+      lc1_src sc1_src mem1_src
+      lc1_tgt sc1_tgt mem1_tgt
+      (NONSYNCH: Memory.nonsynch (Local.promises lc1_src))
+      (LOCAL1: sim_local pview lc1_src (local_relfenced lc1_tgt))
+      (SC1: TimeMap.le sc1_src sc1_tgt)
+      (MEM1: sim_memory mem1_src mem1_tgt)
+      (WF1_SRC: Local.wf lc1_src mem1_src)
+      (WF1_TGT: Local.wf lc1_tgt mem1_tgt):
+  exists lc2_src sc2_src,
+    <<STEP_SRC: Local.fence_step lc1_src sc1_src Ordering.plain Ordering.acqrel lc2_src sc2_src>> /\
+    <<LOCAL2: sim_local pview lc2_src (local_relfenced lc1_tgt)>> /\
+    <<SC2: TimeMap.le sc2_src sc1_tgt>>.
+Proof.
+  inv LOCAL1. inv TVIEW. ss.
+  esplits; eauto.
+  - econs; eauto. i. ss.
+  - econs; eauto. econs; ss; eauto.
+    repeat (condtac; aggrtac).
+Qed.
+
+Lemma sim_local_fence_tgt_relfenced
+      pview
+      lc1_src sc1_src mem1_src
+      lc1_tgt sc1_tgt mem1_tgt
+      lc2_tgt sc2_tgt
+      (STEP_TGT: Local.fence_step lc1_tgt sc1_tgt Ordering.plain Ordering.acqrel lc2_tgt sc2_tgt)
+      (LOCAL1: sim_local pview lc1_src (local_relfenced lc1_tgt))
+      (SC1: TimeMap.le sc1_src sc1_tgt)
+      (MEM1: sim_memory mem1_src mem1_tgt)
+      (WF1_SRC: Local.wf lc1_src mem1_src)
+      (WF1_TGT: Local.wf lc1_tgt mem1_tgt):
+  <<LOCAL2: sim_local SimPromises.bot lc1_src lc2_tgt>> /\
+  <<SC2: TimeMap.le sc1_src sc2_tgt>>.
+Proof.
+  inv LOCAL1. inv TVIEW. inv STEP_TGT. esplits; ss.
+  econs; s.
+  - unfold TView.read_fence_tview. condtac; ss.
+    unfold TView.write_fence_tview. econs; repeat (condtac; aggrtac).
+  - econs; try by apply PROMISES.
+    + inv PROMISES. ii. exploit LE; eauto.
+      SimPromises.none_if_tac.
+      exploit RELEASE; eauto. s. i. subst. ss.
+    + i. rewrite SimPromises.bot_spec in *. congr.
+Qed.
